The coprocessor registers are now modelled with ``:'a ** 16`` instead of ``:cp_register -> 'a``.
Also tidied up and added some proofs about substitutions.

examples/elliptic/arm/arm_evalLib.sig
@@ -9,6 +9,7 @@ sig
    val ARM_RULE             : rule
    val ARM_ASSEMBLE_CONV    : conv
    val SORT_SUBST_CONV      : conv
+   val SORT_FSUBST_CONV     : conv
    val SORT_BSUBST_CONV     : conv
 
    val hol_assemble1        : term -> Arbnum.num -> term frag list -> term
